lib/Word_Lib/Word_Syntax.thy
@@ -8,57 +8,29 @@ section "Additional Syntax for Word Bit Operations"
 
 theory Word_Syntax
 imports
-  "HOL-Word.More_Word"
-  WordBitwise_Signed
-  Hex_Words
-  Norm_Words
-  Word_Type_Syntax
+  "HOL-Library.Word"
 begin
 
 text \<open>Additional bit and type syntax that forces word types.\<close>
 
-type_synonym word8 = "8 word"
-type_synonym word16 = "16 word"
-type_synonym word32 = "32 word"
-type_synonym word64 = "64 word"
-
-lemma len8: "len_of (x :: 8 itself) = 8" by simp
-lemma len16: "len_of (x :: 16 itself) = 16" by simp
-lemma len32: "len_of (x :: 32 itself) = 32" by simp
-lemma len64: "len_of (x :: 64 itself) = 64" by simp
-
-
 abbreviation
-  wordNOT  :: "'a::len0 word \<Rightarrow> 'a word"      ("~~ _" [70] 71)
+  wordNOT  :: "'a::len word \<Rightarrow> 'a word"      ("~~ _" [70] 71)
 where
   "~~ x == NOT x"
 
 abbreviation
-  wordAND  :: "'a::len0 word \<Rightarrow> 'a word \<Rightarrow> 'a word" (infixr "&&" 64)
+  wordAND  :: "'a::len word \<Rightarrow> 'a word \<Rightarrow> 'a word" (infixr "&&" 64)
 where
   "a && b == a AND b"
 
 abbreviation
-  wordOR   :: "'a::len0 word \<Rightarrow> 'a word \<Rightarrow> 'a word" (infixr "||"  59)
+  wordOR   :: "'a::len word \<Rightarrow> 'a word \<Rightarrow> 'a word" (infixr "||"  59)
 where
   "a || b == a OR b"
 
 abbreviation
-  wordXOR  :: "'a::len0 word \<Rightarrow> 'a word \<Rightarrow> 'a word" (infixr "xor" 59)
+  wordXOR  :: "'a::len word \<Rightarrow> 'a word \<Rightarrow> 'a word" (infixr "xor" 59)
 where
   "a xor b == a XOR b"
-
-(* testing for presence of word_bitwise *)
-lemma "((x :: word32) >> 3) AND 7 = (x AND 56) >> 3"
-  by word_bitwise
-
-(* FIXME: move to Word distribution *)
-lemma bin_nth_minus_Bit0[simp]:
-  "0 < n \<Longrightarrow> bin_nth (numeral (num.Bit0 w)) n = bin_nth (numeral w) (n - 1)"
-  by (cases n; simp)
-
-lemma bin_nth_minus_Bit1[simp]:
-  "0 < n \<Longrightarrow> bin_nth (numeral (num.Bit1 w)) n = bin_nth (numeral w) (n - 1)"
-  by (cases n; simp)
 
 end
