lib/Word_Lib/Legacy_Aliases.thy
@@ -1,0 +1,24 @@
+(*
+ * Copyright Data61, CSIRO (ABN 41 687 119 230)
+ *
+ * SPDX-License-Identifier: BSD-2-Clause
+ *)
+
+section \<open>Legacy aliases\<close>
+
+theory Legacy_Aliases
+  imports "HOL-Library.Word"
+begin
+
+definition
+  complement :: "'a :: len word \<Rightarrow> 'a word"  where
+ "complement x \<equiv> NOT x"
+
+lemma complement_mask:
+  "complement (2 ^ n - 1) = NOT (mask n)"
+  unfolding complement_def mask_eq_decr_exp by simp
+
+lemmas less_def = less_eq [symmetric]
+lemmas le_def = not_less [symmetric, where ?'a = nat]
+
+end
