lib/Word_Lib/More_Word.thy
@@ -1,0 +1,1807 @@
+(*
+ * Copyright Data61, CSIRO (ABN 41 687 119 230)
+ *
+ * SPDX-License-Identifier: BSD-2-Clause
+ *)
+
+section \<open>Lemmas on words\<close>
+
+theory More_Word
+  imports
+    "HOL-Library.Word"
+    More_Arithmetic
+    More_Divides
+begin
+
+lemma unat_power_lower [simp]:
+  "unat ((2::'a::len word) ^ n) = 2 ^ n" if "n < LENGTH('a::len)"
+  using that by transfer simp
+
+lemma unat_p2: "n < LENGTH('a :: len) \<Longrightarrow> unat (2 ^ n :: 'a word) = 2 ^ n"
+  by (fact unat_power_lower)
+
+lemma word_div_lt_eq_0:
+  "x < y \<Longrightarrow> x div y = 0" for x :: "'a :: len word"
+  by transfer simp
+
+lemma word_div_eq_1_iff: "n div m = 1 \<longleftrightarrow> n \<ge> m \<and> unat n < 2 * unat (m :: 'a :: len word)"
+  apply (simp only: word_arith_nat_defs word_le_nat_alt word_of_nat_eq_iff flip: nat_div_eq_Suc_0_iff)
+  apply (simp flip: unat_div unsigned_take_bit_eq)
+  done
+
+lemma shiftl_power:
+  "(shiftl1 ^^ x) (y::'a::len word) = 2 ^ x * y"
+  apply (induct x)
+   apply simp
+  apply (simp add: shiftl1_2t)
+  done
+
+lemma AND_twice [simp]:
+  "(w AND m) AND m = w AND m"
+  by (fact and.right_idem)
+
+lemma word_combine_masks:
+  "w AND m = z \<Longrightarrow> w AND m' = z' \<Longrightarrow> w AND (m OR m') = (z OR z')"
+  for w m m' z z' :: \<open>'a::len word\<close>
+  by (simp add: bit.conj_disj_distrib)
+
+lemma p2_gt_0:
+  "(0 < (2 ^ n :: 'a :: len word)) = (n < LENGTH('a))"
+  by (simp add : word_gt_0 not_le)
+
+lemma uint_2p_alt:
+  \<open>n < LENGTH('a::len) \<Longrightarrow> uint ((2::'a::len word) ^ n) = 2 ^ n\<close>
+  using p2_gt_0 [of n, where ?'a = 'a] by (simp add: uint_2p)
+
+lemma p2_eq_0:
+  \<open>(2::'a::len word) ^ n = 0 \<longleftrightarrow> LENGTH('a::len) \<le> n\<close>
+  by (fact exp_eq_zero_iff)
+
+lemma p2len:
+  \<open>(2 :: 'a word) ^ LENGTH('a::len) = 0\<close>
+  by simp
+
+lemma neg_mask_is_div:
+  "w AND NOT (mask n) = (w div 2^n) * 2^n"
+  for w :: \<open>'a::len word\<close>
+  by (rule bit_word_eqI)
+    (auto simp add: bit_simps simp flip: push_bit_eq_mult drop_bit_eq_div)
+
+lemma neg_mask_is_div':
+  "n < size w \<Longrightarrow> w AND NOT (mask n) = ((w div (2 ^ n)) * (2 ^ n))"
+  for w :: \<open>'a::len word\<close>
+  by (rule neg_mask_is_div)
+
+lemma and_mask_arith:
+  "w AND mask n = (w * 2^(size w - n)) div 2^(size w - n)"
+  for w :: \<open>'a::len word\<close>
+  by (rule bit_word_eqI)
+    (auto simp add: bit_simps word_size simp flip: push_bit_eq_mult drop_bit_eq_div)
+
+lemma and_mask_arith':
+  "0 < n \<Longrightarrow> w AND mask n = (w * 2^(size w - n)) div 2^(size w - n)"
+  for w :: \<open>'a::len word\<close>
+  by (rule and_mask_arith)
+
+lemma mask_2pm1: "mask n = 2 ^ n - (1 :: 'a::len word)"
+  by (fact mask_eq_decr_exp)
+
+lemma add_mask_fold:
+  "x + 2 ^ n - 1 = x + mask n"
+  for x :: \<open>'a::len word\<close>
+  by (simp add: mask_eq_decr_exp)
+
+lemma word_and_mask_le_2pm1: "w AND mask n \<le> 2 ^ n - 1"
+  for w :: \<open>'a::len word\<close>
+  by (simp add: mask_2pm1[symmetric] word_and_le1)
+
+lemma is_aligned_AND_less_0:
+  "u AND mask n = 0 \<Longrightarrow> v < 2^n \<Longrightarrow> u AND v = 0"
+  for u v :: \<open>'a::len word\<close>
+  apply (drule less_mask_eq)
+  apply (simp flip: take_bit_eq_mask)
+  apply (simp add: bit_eq_iff)
+  apply (auto simp add: bit_simps)
+  done
+
+lemma le_shiftr1:
+  \<open>shiftr1 u \<le> shiftr1 v\<close> if \<open>u \<le> v\<close>
+using that proof transfer
+  fix k l :: int
+  assume \<open>take_bit LENGTH('a) k \<le> take_bit LENGTH('a) l\<close>
+  then have \<open>take_bit LENGTH('a) (drop_bit 1 (take_bit LENGTH('a) k))
+    \<le> take_bit LENGTH('a) (drop_bit 1 (take_bit LENGTH('a) l))\<close>
+    apply (simp add: take_bit_drop_bit min_def)
+    apply (simp add: drop_bit_eq_div)
+    done
+  then show \<open>take_bit LENGTH('a) (take_bit LENGTH('a) k div 2)
+    \<le> take_bit LENGTH('a) (take_bit LENGTH('a) l div 2)\<close>
+    by (simp add: drop_bit_eq_div)
+qed
+
+lemma and_mask_eq_iff_le_mask:
+  \<open>w AND mask n = w \<longleftrightarrow> w \<le> mask n\<close>
+  for w :: \<open>'a::len word\<close>
+  apply (simp flip: take_bit_eq_mask)
+  apply (cases \<open>n \<ge> LENGTH('a)\<close>; transfer)
+   apply (simp_all add: not_le min_def)
+   apply (simp_all add: mask_eq_exp_minus_1)
+  apply auto
+   apply (metis take_bit_int_less_exp)
+  apply (metis min_def nat_less_le take_bit_int_eq_self_iff take_bit_take_bit)
+  done
+
+lemma less_eq_mask_iff_take_bit_eq_self:
+  \<open>w \<le> mask n \<longleftrightarrow> take_bit n w = w\<close>
+  for w :: \<open>'a::len word\<close>
+  by (simp add: and_mask_eq_iff_le_mask take_bit_eq_mask)
+
+lemma NOT_eq:
+  "NOT (x :: 'a :: len word) = - x - 1"
+  apply (cut_tac x = "x" in word_add_not)
+  apply (drule add.commute [THEN trans])
+  apply (drule eq_diff_eq [THEN iffD2])
+  by simp
+
+lemma NOT_mask: "NOT (mask n :: 'a::len word) = - (2 ^ n)"
+  by (simp add : NOT_eq mask_2pm1)
+
+lemma le_m1_iff_lt: "(x > (0 :: 'a :: len word)) = ((y \<le> x - 1) = (y < x))"
+  by uint_arith
+
+lemma gt0_iff_gem1:
+  \<open>0 < x \<longleftrightarrow> x - 1 < x\<close>
+  for x :: \<open>'a::len word\<close>
+  by (metis add.right_neutral diff_add_cancel less_irrefl measure_unat unat_arith_simps(2) word_neq_0_conv word_sub_less_iff)
+
+lemma power_2_ge_iff:
+  \<open>2 ^ n - (1 :: 'a::len word) < 2 ^ n \<longleftrightarrow> n < LENGTH('a)\<close>
+  using gt0_iff_gem1 p2_gt_0 by blast
+
+lemma le_mask_iff_lt_2n:
+  "n < len_of TYPE ('a) = (((w :: 'a :: len word) \<le> mask n) = (w < 2 ^ n))"
+  unfolding mask_2pm1 by (rule trans [OF p2_gt_0 [THEN sym] le_m1_iff_lt])
+
+lemma mask_lt_2pn:
+  \<open>n < LENGTH('a) \<Longrightarrow> mask n < (2 :: 'a::len word) ^ n\<close>
+  by (simp add: mask_eq_exp_minus_1 power_2_ge_iff)
+
+lemma word_unat_power:
+  "(2 :: 'a :: len word) ^ n = of_nat (2 ^ n)"
+  by simp
+
+lemma of_nat_mono_maybe:
+  assumes xlt: "x < 2 ^ len_of TYPE ('a)"
+  shows   "y < x \<Longrightarrow> of_nat y < (of_nat x :: 'a :: len word)"
+  apply (subst word_less_nat_alt)
+  apply (subst unat_of_nat)+
+  apply (subst mod_less)
+   apply (erule order_less_trans [OF _ xlt])
+  apply (subst mod_less [OF xlt])
+  apply assumption
+  done
+
+lemma word_and_max_word:
+  fixes a::"'a::len word"
+  shows "x = max_word \<Longrightarrow> a AND x = a"
+  by simp
+
+lemma word_and_full_mask_simp:
+  \<open>x AND mask LENGTH('a) = x\<close> for x :: \<open>'a::len word\<close>
+proof (rule bit_eqI)
+  fix n
+  assume \<open>2 ^ n \<noteq> (0 :: 'a word)\<close>
+  then have \<open>n < LENGTH('a)\<close>
+    by simp
+  then show \<open>bit (x AND Bit_Operations.mask LENGTH('a)) n \<longleftrightarrow> bit x n\<close>
+    by (simp add: bit_and_iff bit_mask_iff)
+qed
+
+lemma of_int_uint:
+  "of_int (uint x) = x"
+  by (fact word_of_int_uint)
+
+corollary word_plus_and_or_coroll:
+  "x AND y = 0 \<Longrightarrow> x + y = x OR y"
+  for x y :: \<open>'a::len word\<close>
+  using word_plus_and_or[where x=x and y=y]
+  by simp
+
+corollary word_plus_and_or_coroll2:
+  "(x AND w) + (x AND NOT w) = x"
+  for x w :: \<open>'a::len word\<close>
+  apply (subst disjunctive_add)
+   apply (simp add: bit_simps)
+  apply (simp flip: bit.conj_disj_distrib)
+  done
+
+lemma nat_mask_eq:
+  \<open>nat (mask n) = mask n\<close>
+  by (simp add: nat_eq_iff of_nat_mask_eq)
+
+lemma unat_mask_eq:
+  \<open>unat (mask n :: 'a::len word) = mask (min LENGTH('a) n)\<close>
+  by transfer (simp add: nat_mask_eq)
+
+lemma word_plus_mono_left:
+  fixes x :: "'a :: len word"
+  shows "\<lbrakk>y \<le> z; x \<le> x + z\<rbrakk> \<Longrightarrow> y + x \<le> z + x"
+  by unat_arith
+
+lemma less_Suc_unat_less_bound:
+  "n < Suc (unat (x :: 'a :: len word)) \<Longrightarrow> n < 2 ^ LENGTH('a)"
+  by (auto elim!: order_less_le_trans intro: Suc_leI)
+
+lemma up_ucast_inj:
+  "\<lbrakk> ucast x = (ucast y::'b::len word); LENGTH('a) \<le> len_of TYPE ('b) \<rbrakk> \<Longrightarrow> x = (y::'a::len word)"
+  by transfer (simp add: min_def split: if_splits)
+
+lemmas ucast_up_inj = up_ucast_inj
+
+lemma up_ucast_inj_eq:
+  "LENGTH('a) \<le> len_of TYPE ('b) \<Longrightarrow> (ucast x = (ucast y::'b::len word)) = (x = (y::'a::len word))"
+  by (fastforce dest: up_ucast_inj)
+
+lemma no_plus_overflow_neg:
+  "(x :: 'a :: len word) < -y \<Longrightarrow> x \<le> x + y"
+  by (metis diff_minus_eq_add less_imp_le sub_wrap_lt)
+
+lemma ucast_ucast_eq:
+  "\<lbrakk> ucast x = (ucast (ucast y::'a word)::'c::len word); LENGTH('a) \<le> LENGTH('b);
+     LENGTH('b) \<le> LENGTH('c) \<rbrakk> \<Longrightarrow>
+   x = ucast y" for x :: "'a::len word" and y :: "'b::len word"
+  apply transfer
+  apply (cases \<open>LENGTH('c) = LENGTH('a)\<close>)
+   apply (auto simp add: min_def)
+  done
+
+lemma ucast_0_I:
+  "x = 0 \<Longrightarrow> ucast x = 0"
+  by simp
+
+lemma word_add_offset_less:
+  fixes x :: "'a :: len word"
+  assumes yv: "y < 2 ^ n"
+  and     xv: "x < 2 ^ m"
+  and     mnv: "sz < LENGTH('a :: len)"
+  and    xv': "x < 2 ^ (LENGTH('a :: len) - n)"
+  and     mn: "sz = m + n"
+  shows   "x * 2 ^ n + y < 2 ^ sz"
+proof (subst mn)
+  from mnv mn have nv: "n < LENGTH('a)" and mv: "m < LENGTH('a)"  by auto
+
+  have uy: "unat y < 2 ^ n"
+    by (rule order_less_le_trans [OF unat_mono [OF yv] order_eq_refl],
+        rule unat_power_lower[OF nv])
+
+  have ux: "unat x < 2 ^ m"
+    by (rule order_less_le_trans [OF unat_mono [OF xv] order_eq_refl],
+        rule unat_power_lower[OF mv])
+
+  then show "x * 2 ^ n + y < 2 ^ (m + n)" using ux uy nv mnv xv'
+    apply (subst word_less_nat_alt)
+    apply (subst unat_word_ariths)+
+    apply (subst mod_less)
+     apply simp
+     apply (subst mult.commute)
+     apply (rule nat_less_power_trans [OF _ order_less_imp_le [OF nv]])
+     apply (rule order_less_le_trans [OF unat_mono [OF xv']])
+     apply (cases "n = 0"; simp)
+    apply (subst unat_power_lower[OF nv])
+    apply (subst mod_less)
+     apply (erule order_less_le_trans [OF nat_add_offset_less], assumption)
+      apply (rule mn)
+     apply simp
+    apply (simp add: mn mnv)
+    apply (erule nat_add_offset_less; simp)
+    done
+qed
+
+lemma word_less_power_trans:
+  fixes n :: "'a :: len word"
+  assumes nv: "n < 2 ^ (m - k)"
+  and     kv: "k \<le> m"
+  and     mv: "m < len_of TYPE ('a)"
+  shows "2 ^ k * n < 2 ^ m"
+  using nv kv mv
+  apply -
+  apply (subst word_less_nat_alt)
+  apply (subst unat_word_ariths)
+  apply (subst mod_less)
+   apply simp
+   apply (rule nat_less_power_trans)
+    apply (erule order_less_trans [OF unat_mono])
+    apply simp
+   apply simp
+  apply simp
+  apply (rule nat_less_power_trans)
+   apply (subst unat_power_lower[where 'a = 'a, symmetric])
+    apply simp
+   apply (erule unat_mono)
+  apply simp
+  done
+
+lemma  word_less_power_trans2:
+  fixes n :: "'a::len word"
+  shows "\<lbrakk>n < 2 ^ (m - k); k \<le> m; m < LENGTH('a)\<rbrakk> \<Longrightarrow> n * 2 ^ k < 2 ^ m"
+  by (subst field_simps, rule word_less_power_trans)
+
+lemma Suc_unat_diff_1:
+  fixes x :: "'a :: len word"
+  assumes lt: "1 \<le> x"
+  shows "Suc (unat (x - 1)) = unat x"
+proof -
+  have "0 < unat x"
+    by (rule order_less_le_trans [where y = 1], simp, subst unat_1 [symmetric],
+        rule iffD1 [OF word_le_nat_alt lt])
+
+  then show ?thesis
+    by ((subst unat_sub [OF lt])+, simp only:  unat_1)
+qed
+
+lemma word_eq_unatI:
+  \<open>v = w\<close> if \<open>unat v = unat w\<close>
+  using that by transfer (simp add: nat_eq_iff)
+
+lemma word_div_sub:
+  fixes x :: "'a :: len word"
+  assumes yx: "y \<le> x"
+  and     y0: "0 < y"
+  shows "(x - y) div y = x div y - 1"
+  apply (rule word_eq_unatI)
+  apply (subst unat_div)
+  apply (subst unat_sub [OF yx])
+  apply (subst unat_sub)
+   apply (subst word_le_nat_alt)
+   apply (subst unat_div)
+   apply (subst le_div_geq)
+     apply (rule order_le_less_trans [OF _ unat_mono [OF y0]])
+     apply simp
+    apply (subst word_le_nat_alt [symmetric], rule yx)
+   apply simp
+  apply (subst unat_div)
+  apply (subst le_div_geq [OF _ iffD1 [OF word_le_nat_alt yx]])
+   apply (rule order_le_less_trans [OF _ unat_mono [OF y0]])
+   apply simp
+  apply simp
+  done
+
+lemma word_mult_less_mono1:
+  fixes i :: "'a :: len word"
+  assumes ij: "i < j"
+  and    knz: "0 < k"
+  and    ujk: "unat j * unat k < 2 ^ len_of TYPE ('a)"
+  shows  "i * k < j * k"
+proof -
+  from ij ujk knz have jk: "unat i * unat k < 2 ^ len_of TYPE ('a)"
+    by (auto intro: order_less_subst2 simp: word_less_nat_alt elim: mult_less_mono1)
+
+  then show ?thesis using ujk knz ij
+    by (auto simp: word_less_nat_alt iffD1 [OF unat_mult_lem])
+qed
+
+lemma word_mult_less_dest:
+  fixes i :: "'a :: len word"
+  assumes ij: "i * k < j * k"
+  and    uik: "unat i * unat k < 2 ^ len_of TYPE ('a)"
+  and    ujk: "unat j * unat k < 2 ^ len_of TYPE ('a)"
+  shows  "i < j"
+  using uik ujk ij
+  by (auto simp: word_less_nat_alt iffD1 [OF unat_mult_lem] elim: mult_less_mono1)
+
+lemma word_mult_less_cancel:
+  fixes k :: "'a :: len word"
+  assumes knz: "0 < k"
+  and    uik: "unat i * unat k < 2 ^ len_of TYPE ('a)"
+  and    ujk: "unat j * unat k < 2 ^ len_of TYPE ('a)"
+  shows "(i * k < j * k) = (i < j)"
+  by (rule iffI [OF word_mult_less_dest [OF _ uik ujk] word_mult_less_mono1 [OF _ knz ujk]])
+
+lemma Suc_div_unat_helper:
+  assumes szv: "sz < LENGTH('a :: len)"
+  and   usszv: "us \<le> sz"
+  shows "2 ^ (sz - us) = Suc (unat (((2::'a :: len word) ^ sz - 1) div 2 ^ us))"
+proof -
+  note usv = order_le_less_trans [OF usszv szv]
+
+  from usszv obtain q where qv: "sz = us + q" by (auto simp: le_iff_add)
+
+  have "Suc (unat (((2:: 'a word) ^ sz - 1) div 2 ^ us)) =
+    (2 ^ us + unat ((2:: 'a word) ^ sz - 1)) div 2 ^ us"
+    apply (subst unat_div unat_power_lower[OF usv])+
+    apply (subst div_add_self1, simp+)
+    done
+
+  also have "\<dots> = ((2 ^ us - 1) + 2 ^ sz) div 2 ^ us" using szv
+    by (simp add: unat_minus_one)
+
+  also have "\<dots> = 2 ^ q + ((2 ^ us - 1) div 2 ^ us)"
+    apply (subst qv)
+    apply (subst power_add)
+    apply (subst div_mult_self2; simp)
+    done
+
+  also have "\<dots> = 2 ^ (sz - us)" using qv by simp
+
+  finally show ?thesis ..
+qed
+
+lemma enum_word_nth_eq:
+  \<open>(Enum.enum :: 'a::len word list) ! n = word_of_nat n\<close>
+    if \<open>n < 2 ^ LENGTH('a)\<close>
+    for n
+  using that by (simp add: enum_word_def)
+
+lemma length_enum_word_eq:
+  \<open>length (Enum.enum :: 'a::len word list) = 2 ^ LENGTH('a)\<close>
+  by (simp add: enum_word_def)
+
+lemma unat_lt2p [iff]:
+  \<open>unat x < 2 ^ LENGTH('a)\<close> for x :: \<open>'a::len word\<close>
+  by transfer simp
+
+lemma of_nat_unat [simp]:
+  "of_nat \<circ> unat = id"
+  by (rule ext, simp)
+
+lemma Suc_unat_minus_one [simp]:
+  "x \<noteq> 0 \<Longrightarrow> Suc (unat (x - 1)) = unat x"
+  by (metis Suc_diff_1 unat_gt_0 unat_minus_one)
+
+lemma word_add_le_dest:
+  fixes i :: "'a :: len word"
+  assumes le: "i + k \<le> j + k"
+  and    uik: "unat i + unat k < 2 ^ len_of TYPE ('a)"
+  and    ujk: "unat j + unat k < 2 ^ len_of TYPE ('a)"
+  shows  "i \<le> j"
+  using uik ujk le
+  by (auto simp: word_le_nat_alt iffD1 [OF unat_add_lem] elim: add_le_mono1)
+
+lemma word_add_le_mono1:
+  fixes i :: "'a :: len word"
+  assumes ij: "i \<le> j"
+  and    ujk: "unat j + unat k < 2 ^ len_of TYPE ('a)"
+  shows  "i + k \<le> j + k"
+proof -
+  from ij ujk have jk: "unat i + unat k < 2 ^ len_of TYPE ('a)"
+    by (auto elim: order_le_less_subst2 simp: word_le_nat_alt elim: add_le_mono1)
+
+  then show ?thesis using ujk ij
+    by (auto simp: word_le_nat_alt iffD1 [OF unat_add_lem])
+qed
+
+lemma word_add_le_mono2:
+  fixes i :: "'a :: len word"
+  shows "\<lbrakk>i \<le> j; unat j + unat k < 2 ^ LENGTH('a)\<rbrakk> \<Longrightarrow> k + i \<le> k + j"
+  by (subst field_simps, subst field_simps, erule (1) word_add_le_mono1)
+
+lemma word_add_le_iff:
+  fixes i :: "'a :: len word"
+  assumes uik: "unat i + unat k < 2 ^ len_of TYPE ('a)"
+  and     ujk: "unat j + unat k < 2 ^ len_of TYPE ('a)"
+  shows  "(i + k \<le> j + k) = (i \<le> j)"
+proof
+  assume "i \<le> j"
+  show "i + k \<le> j + k" by (rule word_add_le_mono1) fact+
+next
+  assume "i + k \<le> j + k"
+  show "i \<le> j" by (rule word_add_le_dest) fact+
+qed
+
+lemma word_add_less_mono1:
+  fixes i :: "'a :: len word"
+  assumes ij: "i < j"
+  and    ujk: "unat j + unat k < 2 ^ len_of TYPE ('a)"
+  shows  "i + k < j + k"
+proof -
+  from ij ujk have jk: "unat i + unat k < 2 ^ len_of TYPE ('a)"
+    by (auto elim: order_le_less_subst2 simp: word_less_nat_alt elim: add_less_mono1)
+
+  then show ?thesis using ujk ij
+    by (auto simp: word_less_nat_alt iffD1 [OF unat_add_lem])
+qed
+
+lemma word_add_less_dest:
+  fixes i :: "'a :: len word"
+  assumes le: "i + k < j + k"
+  and    uik: "unat i + unat k < 2 ^ len_of TYPE ('a)"
+  and    ujk: "unat j + unat k < 2 ^ len_of TYPE ('a)"
+  shows  "i < j"
+  using uik ujk le
+  by (auto simp: word_less_nat_alt iffD1 [OF unat_add_lem] elim: add_less_mono1)
+
+lemma word_add_less_iff:
+  fixes i :: "'a :: len word"
+  assumes uik: "unat i + unat k < 2 ^ len_of TYPE ('a)"
+  and     ujk: "unat j + unat k < 2 ^ len_of TYPE ('a)"
+  shows  "(i + k < j + k) = (i < j)"
+proof
+  assume "i < j"
+  show "i + k < j + k" by (rule word_add_less_mono1) fact+
+next
+  assume "i + k < j + k"
+  show "i < j" by (rule word_add_less_dest) fact+
+qed
+
+lemma word_mult_less_iff:
+  fixes i :: "'a :: len word"
+  assumes knz: "0 < k"
+  and     uik: "unat i * unat k < 2 ^ len_of TYPE ('a)"
+  and     ujk: "unat j * unat k < 2 ^ len_of TYPE ('a)"
+  shows  "(i * k < j * k) = (i < j)"
+  using assms by (rule word_mult_less_cancel)
+
+lemma word_le_imp_diff_le:
+  fixes n :: "'a::len word"
+  shows "\<lbrakk>k \<le> n; n \<le> m\<rbrakk> \<Longrightarrow> n - k \<le> m"
+  by (auto simp: unat_sub word_le_nat_alt)
+
+lemma word_less_imp_diff_less:
+  fixes n :: "'a::len word"
+  shows "\<lbrakk>k \<le> n; n < m\<rbrakk> \<Longrightarrow> n - k < m"
+  by (clarsimp simp: unat_sub word_less_nat_alt
+             intro!: less_imp_diff_less)
+
+lemma word_mult_le_mono1:
+  fixes i :: "'a :: len word"
+  assumes ij: "i \<le> j"
+  and    knz: "0 < k"
+  and    ujk: "unat j * unat k < 2 ^ len_of TYPE ('a)"
+  shows  "i * k \<le> j * k"
+proof -
+  from ij ujk knz have jk: "unat i * unat k < 2 ^ len_of TYPE ('a)"
+    by (auto elim: order_le_less_subst2 simp: word_le_nat_alt elim: mult_le_mono1)
+
+  then show ?thesis using ujk knz ij
+    by (auto simp: word_le_nat_alt iffD1 [OF unat_mult_lem])
+qed
+
+lemma word_mult_le_iff:
+  fixes i :: "'a :: len word"
+  assumes knz: "0 < k"
+  and     uik: "unat i * unat k < 2 ^ len_of TYPE ('a)"
+  and     ujk: "unat j * unat k < 2 ^ len_of TYPE ('a)"
+  shows  "(i * k \<le> j * k) = (i \<le> j)"
+proof
+  assume "i \<le> j"
+  show "i * k \<le> j * k" by (rule word_mult_le_mono1) fact+
+next
+  assume p: "i * k \<le> j * k"
+
+  have "0 < unat k" using knz by (simp add: word_less_nat_alt)
+  then show "i \<le> j" using p
+    by (clarsimp simp: word_le_nat_alt iffD1 [OF unat_mult_lem uik]
+      iffD1 [OF unat_mult_lem ujk])
+qed
+
+lemma word_diff_less:
+  fixes n :: "'a :: len word"
+  shows "\<lbrakk>0 < n; 0 < m; n \<le> m\<rbrakk> \<Longrightarrow> m - n < m"
+  apply (subst word_less_nat_alt)
+  apply (subst unat_sub)
+   apply assumption
+  apply (rule diff_less)
+   apply (simp_all add: word_less_nat_alt)
+  done
+
+lemma word_add_increasing:
+  fixes x :: "'a :: len word"
+  shows "\<lbrakk> p + w \<le> x; p \<le> p + w \<rbrakk> \<Longrightarrow> p \<le> x"
+  by unat_arith
+
+lemma word_random:
+  fixes x :: "'a :: len word"
+  shows "\<lbrakk> p \<le> p + x'; x \<le> x' \<rbrakk> \<Longrightarrow> p \<le> p + x"
+  by unat_arith
+
+lemma word_sub_mono:
+  "\<lbrakk> a \<le> c; d \<le> b; a - b \<le> a; c - d \<le> c \<rbrakk>
+    \<Longrightarrow> (a - b) \<le> (c - d :: 'a :: len word)"
+  by unat_arith
+
+lemma power_not_zero:
+  "n < LENGTH('a::len) \<Longrightarrow> (2 :: 'a word) ^ n \<noteq> 0"
+  by (metis p2_gt_0 word_neq_0_conv)
+
+lemma word_gt_a_gt_0:
+  "a < n \<Longrightarrow> (0 :: 'a::len word) < n"
+  apply (case_tac "n = 0")
+   apply clarsimp
+  apply (clarsimp simp: word_neq_0_conv)
+  done
+
+lemma word_power_less_1 [simp]:
+  "sz < LENGTH('a::len) \<Longrightarrow> (2::'a word) ^ sz - 1 < 2 ^ sz"
+  apply (simp add: word_less_nat_alt)
+  apply (subst unat_minus_one)
+  apply simp_all
+  done
+
+lemma word_sub_1_le:
+  "x \<noteq> 0 \<Longrightarrow> x - 1 \<le> (x :: ('a :: len) word)"
+  apply (subst no_ulen_sub)
+  apply simp
+  apply (cases "uint x = 0")
+   apply (simp add: uint_0_iff)
+  apply (insert uint_ge_0[where x=x])
+  apply arith
+  done
+
+lemma push_bit_word_eq_nonzero:
+  \<open>push_bit n w \<noteq> 0\<close> if \<open>w < 2 ^ m\<close> \<open>m + n < LENGTH('a)\<close> \<open>w \<noteq> 0\<close>
+    for w :: \<open>'a::len word\<close>
+  using that
+  apply (simp only: word_neq_0_conv word_less_nat_alt
+                    mod_0 unat_word_ariths
+                    unat_power_lower word_le_nat_alt)
+  apply (metis add_diff_cancel_right' gr0I gr_implies_not0 less_or_eq_imp_le min_def push_bit_eq_0_iff take_bit_nat_eq_self_iff take_bit_push_bit take_bit_take_bit unsigned_push_bit_eq)
+  done
+
+lemma unat_less_power:
+  fixes k :: "'a::len word"
+  assumes szv: "sz < LENGTH('a)"
+  and     kv:  "k < 2 ^ sz"
+  shows   "unat k < 2 ^ sz"
+  using szv unat_mono [OF kv] by simp
+
+lemma unat_mult_power_lem:
+  assumes kv: "k < 2 ^ (LENGTH('a::len) - sz)"
+  shows "unat (2 ^ sz * of_nat k :: (('a::len) word)) = 2 ^ sz * k"
+proof (cases \<open>sz < LENGTH('a)\<close>)
+  case True
+  with assms show ?thesis
+    by (simp add: unat_word_ariths take_bit_eq_mod mod_simps)
+      (simp add: take_bit_nat_eq_self_iff nat_less_power_trans flip: take_bit_eq_mod)
+next
+  case False
+  with assms show ?thesis
+    by simp
+qed
+
+lemma word_plus_mcs_4:
+  "\<lbrakk>v + x \<le> w + x; x \<le> v + x\<rbrakk> \<Longrightarrow> v \<le> (w::'a::len word)"
+  by uint_arith
+
+lemma word_plus_mcs_3:
+  "\<lbrakk>v \<le> w; x \<le> w + x\<rbrakk> \<Longrightarrow> v + x \<le> w + (x::'a::len word)"
+  by unat_arith
+
+lemma word_le_minus_one_leq:
+  "x < y \<Longrightarrow> x \<le> y - 1" for x :: "'a :: len word"
+  by transfer (metis le_less_trans less_irrefl take_bit_decr_eq take_bit_nonnegative zle_diff1_eq)
+
+lemma word_less_sub_le[simp]:
+  fixes x :: "'a :: len word"
+  assumes nv: "n < LENGTH('a)"
+  shows "(x \<le> 2 ^ n - 1) = (x < 2 ^ n)"
+  using le_less_trans word_le_minus_one_leq nv power_2_ge_iff by blast
+
+lemma unat_of_nat_len:
+  "x < 2 ^ LENGTH('a) \<Longrightarrow> unat (of_nat x :: 'a::len word) = x"
+  by (simp add: take_bit_nat_eq_self_iff)
+
+lemma unat_of_nat_eq:
+  "x < 2 ^ LENGTH('a) \<Longrightarrow> unat (of_nat x ::'a::len word) = x"
+  by (rule unat_of_nat_len)
+
+lemma unat_eq_of_nat:
+  "n < 2 ^ LENGTH('a) \<Longrightarrow> (unat (x :: 'a::len word) = n) = (x = of_nat n)"
+  by transfer
+    (auto simp add: take_bit_of_nat nat_eq_iff take_bit_nat_eq_self_iff intro: sym)
+
+lemma alignUp_div_helper:
+  fixes a :: "'a::len word"
+  assumes kv: "k < 2 ^ (LENGTH('a) - n)"
+  and     xk: "x = 2 ^ n * of_nat k"
+  and    le: "a \<le> x"
+  and    sz: "n < LENGTH('a)"
+  and   anz: "a mod 2 ^ n \<noteq> 0"
+  shows "a div 2 ^ n < of_nat k"
+proof -
+  have kn: "unat (of_nat k :: 'a word) * unat ((2::'a word) ^ n) < 2 ^ LENGTH('a)"
+    using xk kv sz
+    apply (subst unat_of_nat_eq)
+     apply (erule order_less_le_trans)
+     apply simp
+    apply (subst unat_power_lower, simp)
+    apply (subst mult.commute)
+    apply (rule nat_less_power_trans)
+     apply simp
+    apply simp
+    done
+
+  have "unat a div 2 ^ n * 2 ^ n \<noteq> unat a"
+  proof -
+    have "unat a = unat a div 2 ^ n * 2 ^ n + unat a mod 2 ^ n"
+      by (simp add: div_mult_mod_eq)
+    also have "\<dots> \<noteq> unat a div 2 ^ n * 2 ^ n" using sz anz
+      by (simp add: unat_arith_simps)
+    finally show ?thesis ..
+  qed
+
+  then have "a div 2 ^ n * 2 ^ n < a" using sz anz
+    apply (subst word_less_nat_alt)
+    apply (subst unat_word_ariths)
+    apply (subst unat_div)
+    apply simp
+    apply (rule order_le_less_trans [OF mod_less_eq_dividend])
+    apply (erule order_le_neq_trans [OF div_mult_le])
+    done
+
+  also from xk le have "\<dots> \<le> of_nat k * 2 ^ n" by (simp add: field_simps)
+  finally show ?thesis using sz kv
+    apply -
+    apply (erule word_mult_less_dest [OF _ _ kn])
+    apply (simp add: unat_div)
+    apply (rule order_le_less_trans [OF div_mult_le])
+    apply (rule unat_lt2p)
+    done
+qed
+
+lemma mask_out_sub_mask:
+  "(x AND NOT (mask n)) = x - (x AND (mask n))"
+  for x :: \<open>'a::len word\<close>
+  by (simp add: field_simps word_plus_and_or_coroll2)
+
+lemma subtract_mask:
+  "p - (p AND mask n) = (p AND NOT (mask n))"
+  "p - (p AND NOT (mask n)) = (p AND mask n)"
+  for p :: \<open>'a::len word\<close>
+  by (simp add: field_simps word_plus_and_or_coroll2)+
+
+lemma take_bit_word_eq_self_iff:
+  \<open>take_bit n w = w \<longleftrightarrow> n \<ge> LENGTH('a) \<or> w < 2 ^ n\<close>
+  for w :: \<open>'a::len word\<close>
+  using take_bit_int_eq_self_iff [of n \<open>take_bit LENGTH('a) (uint w)\<close>]
+  by (transfer fixing: n) auto
+
+lemma word_power_increasing:
+  assumes x: "2 ^ x < (2 ^ y::'a::len word)" "x < LENGTH('a::len)" "y < LENGTH('a::len)"
+  shows "x < y" using x
+  using assms by transfer simp
+
+lemma mask_twice:
+  "(x AND mask n) AND mask m = x AND mask (min m n)"
+  for x :: \<open>'a::len word\<close>
+  by (simp flip: take_bit_eq_mask)
+
+lemma plus_one_helper[elim!]:
+  "x < n + (1 :: 'a :: len word) \<Longrightarrow> x \<le> n"
+  apply (simp add: word_less_nat_alt word_le_nat_alt field_simps)
+  apply (case_tac "1 + n = 0")
+   apply simp_all
+  apply (subst(asm) unatSuc, assumption)
+  apply arith
+  done
+
+lemma plus_one_helper2:
+  "\<lbrakk> x \<le> n; n + 1 \<noteq> 0 \<rbrakk> \<Longrightarrow> x < n + (1 :: 'a :: len word)"
+  by (simp add: word_less_nat_alt word_le_nat_alt field_simps
+                unatSuc)
+
+lemma less_x_plus_1:
+  fixes x :: "'a :: len word" shows
+  "x \<noteq> max_word \<Longrightarrow> (y < (x + 1)) = (y < x \<or> y = x)"
+  apply (rule iffI)
+   apply (rule disjCI)
+   apply (drule plus_one_helper)
+   apply simp
+  apply (subgoal_tac "x < x + 1")
+   apply (erule disjE, simp_all)
+  apply (rule plus_one_helper2 [OF order_refl])
+  apply (rule notI, drule max_word_wrap)
+  apply simp
+  done
+
+lemma word_Suc_leq:
+  fixes k::"'a::len word" shows "k \<noteq> max_word \<Longrightarrow> x < k + 1 \<longleftrightarrow> x \<le> k"
+  using less_x_plus_1 word_le_less_eq by auto
+
+lemma word_Suc_le:
+   fixes k::"'a::len word" shows "x \<noteq> max_word \<Longrightarrow> x + 1 \<le> k \<longleftrightarrow> x < k"
+  by (meson not_less word_Suc_leq)
+
+lemma word_lessThan_Suc_atMost:
+  \<open>{..< k + 1} = {..k}\<close> if \<open>k \<noteq> - 1\<close> for k :: \<open>'a::len word\<close>
+  using that by (simp add: lessThan_def atMost_def word_Suc_leq)
+
+lemma word_atLeastLessThan_Suc_atLeastAtMost:
+  \<open>{l ..< u + 1} = {l..u}\<close> if \<open>u \<noteq> - 1\<close> for l :: \<open>'a::len word\<close>
+  using that by (simp add: atLeastAtMost_def atLeastLessThan_def word_lessThan_Suc_atMost)
+
+lemma word_atLeastAtMost_Suc_greaterThanAtMost:
+  \<open>{m<..u} = {m + 1..u}\<close> if \<open>m \<noteq> - 1\<close> for m :: \<open>'a::len word\<close>
+  using that by (simp add: greaterThanAtMost_def greaterThan_def atLeastAtMost_def atLeast_def word_Suc_le)
+
+lemma word_atLeastLessThan_Suc_atLeastAtMost_union:
+  fixes l::"'a::len word"
+  assumes "m \<noteq> max_word" and "l \<le> m" and "m \<le> u"
+  shows "{l..m} \<union> {m+1..u} = {l..u}"
+  proof -
+  from ivl_disj_un_two(8)[OF assms(2) assms(3)] have "{l..u} = {l..m} \<union> {m<..u}" by blast
+  with assms show ?thesis by(simp add: word_atLeastAtMost_Suc_greaterThanAtMost)
+  qed
+
+lemma max_word_less_eq_iff [simp]:
+  \<open>- 1 \<le> w \<longleftrightarrow> w = - 1\<close> for w :: \<open>'a::len word\<close>
+  by (fact word_order.extremum_unique)
+
+lemma word_or_zero:
+  "(a OR b = 0) = (a = 0 \<and> b = 0)"
+  for a b :: \<open>'a::len word\<close>
+  by (fact or_eq_0_iff)
+
+lemma word_2p_mult_inc:
+  assumes x: "2 * 2 ^ n < (2::'a::len word) * 2 ^ m"
+  assumes suc_n: "Suc n < LENGTH('a::len)"
+  shows "2^n < (2::'a::len word)^m"
+  by (smt suc_n le_less_trans lessI nat_less_le nat_mult_less_cancel_disj p2_gt_0
+          power_Suc power_Suc unat_power_lower word_less_nat_alt x)
+
+lemma power_overflow:
+  "n \<ge> LENGTH('a) \<Longrightarrow> 2 ^ n = (0 :: 'a::len word)"
+  by simp
+
+lemmas extra_sle_sless_unfolds [simp] =
+    word_sle_eq[where a=0 and b=1]
+    word_sle_eq[where a=0 and b="numeral n"]
+    word_sle_eq[where a=1 and b=0]
+    word_sle_eq[where a=1 and b="numeral n"]
+    word_sle_eq[where a="numeral n" and b=0]
+    word_sle_eq[where a="numeral n" and b=1]
+    word_sless_alt[where a=0 and b=1]
+    word_sless_alt[where a=0 and b="numeral n"]
+    word_sless_alt[where a=1 and b=0]
+    word_sless_alt[where a=1 and b="numeral n"]
+    word_sless_alt[where a="numeral n" and b=0]
+    word_sless_alt[where a="numeral n" and b=1]
+  for n
+
+lemma word_sint_1:
+  "sint (1::'a::len word) = (if LENGTH('a) = 1 then -1 else 1)"
+  by (fact signed_1)
+
+lemma ucast_of_nat:
+  "is_down (ucast :: 'a :: len word \<Rightarrow> 'b :: len word)
+    \<Longrightarrow> ucast (of_nat n :: 'a word) = (of_nat n :: 'b word)"
+  by transfer simp
+
+lemma scast_1':
+  "(scast (1::'a::len word) :: 'b::len word) =
+   (word_of_int (signed_take_bit (LENGTH('a::len) - Suc 0) (1::int)))"
+  by transfer simp
+
+lemma scast_1:
+  "(scast (1::'a::len word) :: 'b::len word) = (if LENGTH('a) = 1 then -1 else 1)"
+  by (fact signed_1)
+
+lemma unat_minus_one_word:
+  "unat (-1 :: 'a :: len word) = 2 ^ LENGTH('a) - 1"
+  apply (simp only: flip: mask_eq_exp_minus_1)
+  apply transfer
+  apply (simp add: take_bit_minus_one_eq_mask nat_mask_eq)
+  done
+
+lemmas word_diff_ls'' = word_diff_ls [where xa=x and x=x for x]
+lemmas word_diff_ls' = word_diff_ls'' [simplified]
+
+lemmas word_l_diffs' = word_l_diffs [where xa=x and x=x for x]
+lemmas word_l_diffs = word_l_diffs' [simplified]
+
+lemma two_power_increasing:
+  "\<lbrakk> n \<le> m; m < LENGTH('a) \<rbrakk> \<Longrightarrow> (2 :: 'a :: len word) ^ n \<le> 2 ^ m"
+  by (simp add: word_le_nat_alt)
+
+lemma word_leq_le_minus_one:
+  "\<lbrakk> x \<le> y; x \<noteq> 0 \<rbrakk> \<Longrightarrow> x - 1 < (y :: 'a :: len word)"
+  apply (simp add: word_less_nat_alt word_le_nat_alt)
+  apply (subst unat_minus_one)
+   apply assumption
+  apply (cases "unat x")
+   apply (simp add: unat_eq_zero)
+  apply arith
+  done
+
+lemma neg_mask_combine:
+  "NOT(mask a) AND NOT(mask b) = NOT(mask (max a b) :: 'a::len word)"
+  by (rule bit_word_eqI) (auto simp add: bit_simps)
+
+lemma neg_mask_twice:
+  "x AND NOT(mask n) AND NOT(mask m) = x AND NOT(mask (max n m))"
+  for x :: \<open>'a::len word\<close>
+  by (rule bit_word_eqI) (auto simp add: bit_simps)
+
+lemma multiple_mask_trivia:
+  "n \<ge> m \<Longrightarrow> (x AND NOT(mask n)) + (x AND mask n AND NOT(mask m)) = x AND NOT(mask m)"
+  for x :: \<open>'a::len word\<close>
+  apply (rule trans[rotated], rule_tac w="mask n" in word_plus_and_or_coroll2)
+  apply (simp add: word_bw_assocs word_bw_comms word_bw_lcs neg_mask_twice
+                   max_absorb2)
+  done
+
+lemma word_of_nat_less:
+  "\<lbrakk> n < unat x \<rbrakk> \<Longrightarrow> of_nat n < x"
+  apply (simp add: word_less_nat_alt)
+  apply (erule order_le_less_trans[rotated])
+  apply (simp add: take_bit_eq_mod)
+  done
+
+lemma unat_mask:
+  "unat (mask n :: 'a :: len word) = 2 ^ (min n (LENGTH('a))) - 1"
+  apply (subst min.commute)
+  apply (simp add: mask_eq_decr_exp not_less min_def  split: if_split_asm)
+  apply (intro conjI impI)
+   apply (simp add: unat_sub_if_size)
+   apply (simp add: power_overflow word_size)
+  apply (simp add: unat_sub_if_size)
+  done
+
+lemma mask_over_length:
+  "LENGTH('a) \<le> n \<Longrightarrow> mask n = (-1::'a::len word)"
+  by (simp add: mask_eq_decr_exp)
+
+lemma Suc_2p_unat_mask:
+  "n < LENGTH('a) \<Longrightarrow> Suc (2 ^ n * k + unat (mask n :: 'a::len word)) = 2 ^ n * (k+1)"
+  by (simp add: unat_mask)
+
+lemma sint_of_nat_ge_zero:
+  "x < 2 ^ (LENGTH('a) - 1) \<Longrightarrow> sint (of_nat x :: 'a :: len word) \<ge> 0"
+  by (simp add: bit_iff_odd)
+
+lemma int_eq_sint:
+  "x < 2 ^ (LENGTH('a) - 1) \<Longrightarrow> sint (of_nat x :: 'a :: len word) = int x"
+  apply transfer
+  apply (rule signed_take_bit_int_eq_self)
+   apply simp_all
+  apply (metis negative_zle numeral_power_eq_of_nat_cancel_iff)
+  done
+
+lemma sint_of_nat_le:
+  "\<lbrakk> b < 2 ^ (LENGTH('a) - 1); a \<le> b \<rbrakk>
+   \<Longrightarrow> sint (of_nat a :: 'a :: len word) \<le> sint (of_nat b :: 'a :: len word)"
+  apply (cases \<open>LENGTH('a)\<close>)
+  apply simp_all
+  apply transfer
+  apply (subst signed_take_bit_eq_if_positive)
+   apply (simp add: bit_simps)
+  apply (metis bit_take_bit_iff nat_less_le order_less_le_trans take_bit_nat_eq_self_iff)
+  apply (subst signed_take_bit_eq_if_positive)
+    apply (simp add: bit_simps)
+  apply (metis bit_take_bit_iff nat_less_le take_bit_nat_eq_self_iff)
+    apply (simp flip: of_nat_take_bit add: take_bit_nat_eq_self)
+  done
+
+lemma word_le_not_less:
+  "((b::'a::len word) \<le> a) = (\<not>(a < b))"
+  by fastforce
+
+lemma less_is_non_zero_p1:
+  fixes a :: "'a :: len word"
+  shows "a < k \<Longrightarrow> a + 1 \<noteq> 0"
+  apply (erule contrapos_pn)
+  apply (drule max_word_wrap)
+  apply (simp add: not_less)
+  done
+
+lemma unat_add_lem':
+  "(unat x + unat y < 2 ^ LENGTH('a)) \<Longrightarrow>
+    (unat (x + y :: 'a :: len word) = unat x + unat y)"
+  by (subst unat_add_lem[symmetric], assumption)
+
+lemma word_less_two_pow_divI:
+  "\<lbrakk> (x :: 'a::len word) < 2 ^ (n - m); m \<le> n; n < LENGTH('a) \<rbrakk> \<Longrightarrow> x < 2 ^ n div 2 ^ m"
+  apply (simp add: word_less_nat_alt)
+  apply (subst unat_word_ariths)
+  apply (subst mod_less)
+   apply (rule order_le_less_trans [OF div_le_dividend])
+   apply (rule unat_lt2p)
+  apply (simp add: power_sub)
+  done
+
+lemma word_less_two_pow_divD:
+  "\<lbrakk> (x :: 'a::len word) < 2 ^ n div 2 ^ m \<rbrakk>
+     \<Longrightarrow> n \<ge> m \<and> (x < 2 ^ (n - m))"
+  apply (cases "n < LENGTH('a)")
+   apply (cases "m < LENGTH('a)")
+    apply (simp add: word_less_nat_alt)
+    apply (subst(asm) unat_word_ariths)
+    apply (subst(asm) mod_less)
+     apply (rule order_le_less_trans [OF div_le_dividend])
+     apply (rule unat_lt2p)
+    apply (clarsimp dest!: less_two_pow_divD)
+   apply (simp add: power_overflow)
+   apply (simp add: word_div_def)
+  apply (simp add: power_overflow word_div_def)
+  done
+
+lemma of_nat_less_two_pow_div_set:
+  "\<lbrakk> n < LENGTH('a) \<rbrakk> \<Longrightarrow>
+   {x. x < (2 ^ n div 2 ^ m :: 'a::len word)}
+      = of_nat ` {k. k < 2 ^ n div 2 ^ m}"
+  apply (simp add: image_def)
+  apply (safe dest!: word_less_two_pow_divD less_two_pow_divD
+             intro!: word_less_two_pow_divI)
+   apply (rule_tac x="unat x" in exI)
+   apply (simp add: power_sub[symmetric])
+   apply (subst unat_power_lower[symmetric, where 'a='a])
+    apply simp
+   apply (erule unat_mono)
+  apply (subst word_unat_power)
+  apply (rule of_nat_mono_maybe)
+   apply (rule power_strict_increasing)
+    apply simp
+   apply simp
+  apply assumption
+  done
+
+lemma ucast_less:
+  "LENGTH('b) < LENGTH('a) \<Longrightarrow>
+   (ucast (x :: 'b :: len word) :: ('a :: len word)) < 2 ^ LENGTH('b)"
+  by transfer simp
+
+lemma ucast_range_less:
+  "LENGTH('a :: len) < LENGTH('b :: len) \<Longrightarrow>
+   range (ucast :: 'a word \<Rightarrow> 'b word) = {x. x < 2 ^ len_of TYPE ('a)}"
+  apply safe
+   apply (erule ucast_less)
+  apply (simp add: image_def)
+  apply (rule_tac x="ucast x" in exI)
+  apply (rule bit_word_eqI)
+  apply (auto simp add: bit_simps)
+  apply (metis bit_take_bit_iff less_mask_eq not_less take_bit_eq_mask)
+  done
+
+lemma word_power_less_diff:
+  "\<lbrakk>2 ^ n * q < (2::'a::len word) ^ m; q < 2 ^ (LENGTH('a) - n)\<rbrakk> \<Longrightarrow> q < 2 ^ (m - n)"
+  apply (case_tac "m \<ge> LENGTH('a)")
+   apply (simp add: power_overflow)
+  apply (case_tac "n \<ge> LENGTH('a)")
+   apply (simp add: power_overflow)
+  apply (cases "n = 0")
+   apply simp
+  apply (subst word_less_nat_alt)
+  apply (subst unat_power_lower)
+   apply simp
+  apply (rule nat_power_less_diff)
+  apply (simp add: word_less_nat_alt)
+  apply (subst (asm) iffD1 [OF unat_mult_lem])
+   apply (simp add:nat_less_power_trans)
+  apply simp
+  done
+
+lemma word_less_sub_1:
+  "x < (y :: 'a :: len word) \<Longrightarrow> x \<le> y - 1"
+  by (fact word_le_minus_one_leq)
+
+lemma word_sub_mono2:
+  "\<lbrakk> a + b \<le> c + d; c \<le> a; b \<le> a + b; d \<le> c + d \<rbrakk>
+    \<Longrightarrow> b \<le> (d :: 'a :: len word)"
+  apply (drule(1) word_sub_mono)
+    apply simp
+   apply simp
+  apply simp
+  done
+
+lemma word_not_le:
+  "(\<not> x \<le> (y :: 'a :: len word)) = (y < x)"
+  by fastforce
+
+lemma word_subset_less:
+  "\<lbrakk> {x .. x + r - 1} \<subseteq> {y .. y + s - 1};
+     x \<le> x + r - 1; y \<le> y + (s :: 'a :: len word) - 1;
+     s \<noteq> 0 \<rbrakk>
+     \<Longrightarrow> r \<le> s"
+  apply (frule subsetD[where c=x])
+   apply simp
+  apply (drule subsetD[where c="x + r - 1"])
+   apply simp
+  apply (clarsimp simp: add_diff_eq[symmetric])
+  apply (drule(1) word_sub_mono2)
+    apply (simp_all add: olen_add_eqv[symmetric])
+  apply (erule word_le_minus_cancel)
+  apply (rule ccontr)
+  apply (simp add: word_not_le)
+  done
+
+lemma uint_power_lower:
+  "n < LENGTH('a) \<Longrightarrow> uint (2 ^ n :: 'a :: len word) = (2 ^ n :: int)"
+  by (rule uint_2p_alt)
+
+lemma power_le_mono:
+  "\<lbrakk>2 ^ n \<le> (2::'a::len word) ^ m; n < LENGTH('a); m < LENGTH('a)\<rbrakk>
+   \<Longrightarrow> n \<le> m"
+  apply (clarsimp simp add: le_less)
+  apply safe
+  apply (simp add: word_less_nat_alt)
+  apply (simp only: uint_arith_simps(3))
+  apply (drule uint_power_lower)+
+  apply simp
+  done
+
+lemma two_power_eq:
+  "\<lbrakk>n < LENGTH('a); m < LENGTH('a)\<rbrakk>
+   \<Longrightarrow> ((2::'a::len word) ^ n = 2 ^ m) = (n = m)"
+  apply safe
+  apply (rule order_antisym)
+   apply (simp add: power_le_mono[where 'a='a])+
+  done
+
+lemma unat_less_helper:
+  "x < of_nat n \<Longrightarrow> unat x < n"
+  apply (simp add: word_less_nat_alt)
+  apply (erule order_less_le_trans)
+  apply (simp add: take_bit_eq_mod)
+  done
+
+lemma nat_uint_less_helper:
+  "nat (uint y) = z \<Longrightarrow> x < y \<Longrightarrow> nat (uint x) < z"
+  apply (erule subst)
+  apply (subst unat_eq_nat_uint [symmetric])
+  apply (subst unat_eq_nat_uint [symmetric])
+  by (simp add: unat_mono)
+
+lemma of_nat_0:
+  "\<lbrakk>of_nat n = (0::'a::len word); n < 2 ^ LENGTH('a)\<rbrakk> \<Longrightarrow> n = 0"
+  by transfer (simp add: take_bit_eq_mod)
+
+lemma of_nat_inj:
+  "\<lbrakk>x < 2 ^ LENGTH('a); y < 2 ^ LENGTH('a)\<rbrakk> \<Longrightarrow>
+   (of_nat x = (of_nat y :: 'a :: len word)) = (x = y)"
+  by (metis unat_of_nat_len)
+
+lemma div_to_mult_word_lt:
+  "\<lbrakk> (x :: 'a :: len word) \<le> y div z \<rbrakk> \<Longrightarrow> x * z \<le> y"
+  apply (cases "z = 0")
+   apply simp
+  apply (simp add: word_neq_0_conv)
+  apply (rule order_trans)
+   apply (erule(1) word_mult_le_mono1)
+   apply (simp add: unat_div)
+   apply (rule order_le_less_trans [OF div_mult_le])
+   apply simp
+  apply (rule word_div_mult_le)
+  done
+
+lemma ucast_ucast_mask:
+  "(ucast :: 'a :: len word \<Rightarrow> 'b :: len word) (ucast x) = x AND mask (len_of TYPE ('a))"
+  apply (simp flip: take_bit_eq_mask)
+  apply transfer
+  apply (simp add: ac_simps)
+  done
+
+lemma ucast_ucast_len:
+  "\<lbrakk> x < 2 ^ LENGTH('b) \<rbrakk> \<Longrightarrow> ucast (ucast x::'b::len word) = (x::'a::len word)"
+  apply (subst ucast_ucast_mask)
+  apply (erule less_mask_eq)
+  done
+
+lemma ucast_ucast_id:
+  "LENGTH('a) < LENGTH('b) \<Longrightarrow> ucast (ucast (x::'a::len word)::'b::len word) = x"
+  by (auto intro: ucast_up_ucast_id simp: is_up_def source_size_def target_size_def word_size)
+
+lemma unat_ucast:
+  "unat (ucast x :: ('a :: len) word) = unat x mod 2 ^ (LENGTH('a))"
+proof -
+  have \<open>2 ^ LENGTH('a) = nat (2 ^ LENGTH('a))\<close>
+    by simp
+  moreover have \<open>unat (ucast x :: 'a word) = unat x mod nat (2 ^ LENGTH('a))\<close>
+    by transfer (simp flip: nat_mod_distrib take_bit_eq_mod)
+  ultimately show ?thesis
+    by (simp only:)
+qed
+
+lemma ucast_less_ucast:
+  "LENGTH('a) \<le> LENGTH('b) \<Longrightarrow>
+   (ucast x < ((ucast (y :: 'a::len word)) :: 'b::len word)) = (x < y)"
+  apply (simp add: word_less_nat_alt unat_ucast)
+  apply (subst mod_less)
+   apply(rule less_le_trans[OF unat_lt2p], simp)
+  apply (subst mod_less)
+   apply(rule less_le_trans[OF unat_lt2p], simp)
+  apply simp
+  done
+
+\<comment> \<open>This weaker version was previously called @{text ucast_less_ucast}. We retain it to
+    support existing proofs.\<close>
+lemmas ucast_less_ucast_weak = ucast_less_ucast[OF order.strict_implies_order]
+
+lemma unat_Suc2:
+  fixes n :: "'a :: len word"
+  shows
+  "n \<noteq> -1 \<Longrightarrow> unat (n + 1) = Suc (unat n)"
+  apply (subst add.commute, rule unatSuc)
+  apply (subst eq_diff_eq[symmetric], simp add: minus_equation_iff)
+  done
+
+lemma word_div_1:
+  "(n :: 'a :: len word) div 1 = n"
+  by (fact bits_div_by_1)
+
+lemma word_minus_one_le:
+  "-1 \<le> (x :: 'a :: len word) = (x = -1)"
+  by (fact word_order.extremum_unique)
+
+lemma up_scast_inj:
+      "\<lbrakk> scast x = (scast y :: 'b :: len word); size x \<le> LENGTH('b) \<rbrakk>
+         \<Longrightarrow> x = y"
+  apply transfer
+  apply (cases \<open>LENGTH('a)\<close>)
+  apply simp_all
+  apply (metis order_refl take_bit_signed_take_bit take_bit_tightened)
+  done
+
+lemma up_scast_inj_eq:
+  "LENGTH('a) \<le> len_of TYPE ('b) \<Longrightarrow>
+  (scast x = (scast y::'b::len word)) = (x = (y::'a::len word))"
+  by (fastforce dest: up_scast_inj simp: word_size)
+
+lemma word_le_add:
+  fixes x :: "'a :: len word"
+  shows "x \<le> y \<Longrightarrow> \<exists>n. y = x + of_nat n"
+  by (rule exI [where x = "unat (y - x)"]) simp
+
+lemma word_plus_mcs_4':
+  fixes x :: "'a :: len word"
+  shows "\<lbrakk>x + v \<le> x + w; x \<le> x + v\<rbrakk> \<Longrightarrow> v \<le> w"
+  apply (rule word_plus_mcs_4)
+   apply (simp add: add.commute)
+  apply (simp add: add.commute)
+  done
+
+lemma unat_eq_1:
+  \<open>unat x = Suc 0 \<longleftrightarrow> x = 1\<close>
+  by (auto intro!: unsigned_word_eqI [where ?'a = nat])
+
+lemma word_unat_Rep_inject1:
+  \<open>unat x = unat 1 \<longleftrightarrow> x = 1\<close>
+  by (simp add: unat_eq_1)
+
+lemma and_not_mask_twice:
+  "(w AND NOT (mask n)) AND NOT (mask m) = w AND NOT (mask (max m n))"
+  for w :: \<open>'a::len word\<close>
+  by (rule bit_word_eqI) (auto simp add: bit_simps)
+
+lemma word_less_cases:
+  "x < y \<Longrightarrow> x = y - 1 \<or> x < y - (1 ::'a::len word)"
+  apply (drule word_less_sub_1)
+  apply (drule order_le_imp_less_or_eq)
+  apply auto
+  done
+
+lemma mask_and_mask:
+  "mask a AND mask b = (mask (min a b) :: 'a::len word)"
+  by (simp flip: take_bit_eq_mask ac_simps)
+
+lemma mask_eq_0_eq_x:
+  "(x AND w = 0) = (x AND NOT w = x)"
+  for x w :: \<open>'a::len word\<close>
+  using word_plus_and_or_coroll2[where x=x and w=w]
+  by auto
+
+lemma mask_eq_x_eq_0:
+  "(x AND w = x) = (x AND NOT w = 0)"
+  for x w :: \<open>'a::len word\<close>
+  using word_plus_and_or_coroll2[where x=x and w=w]
+  by auto
+
+lemma compl_of_1: "NOT 1 = (-2 :: 'a :: len word)"
+  by (fact not_one)
+
+lemma split_word_eq_on_mask:
+  "(x = y) = (x AND m = y AND m \<and> x AND NOT m = y AND NOT m)"
+  for x y m :: \<open>'a::len word\<close>
+  apply transfer
+  apply (simp add: bit_eq_iff)
+  apply (auto simp add: bit_simps ac_simps)
+  done
+
+lemma word_FF_is_mask:
+  "0xFF = (mask 8 :: 'a::len word)"
+  by (simp add: mask_eq_decr_exp)
+
+lemma word_1FF_is_mask:
+  "0x1FF = (mask 9 :: 'a::len word)"
+  by (simp add: mask_eq_decr_exp)
+
+lemma ucast_of_nat_small:
+  "x < 2 ^ LENGTH('a) \<Longrightarrow> ucast (of_nat x :: 'a :: len word) = (of_nat x :: 'b :: len word)"
+  apply transfer
+  apply (auto simp add: take_bit_of_nat min_def not_le)
+  apply (metis linorder_not_less min_def take_bit_nat_eq_self take_bit_take_bit)
+  done
+
+lemma word_le_make_less:
+  fixes x :: "'a :: len word"
+  shows "y \<noteq> -1 \<Longrightarrow> (x \<le> y) = (x < (y + 1))"
+  apply safe
+  apply (erule plus_one_helper2)
+  apply (simp add: eq_diff_eq[symmetric])
+  done
+
+lemmas finite_word = finite [where 'a="'a::len word"]
+
+lemma word_to_1_set:
+  "{0 ..< (1 :: 'a :: len word)} = {0}"
+  by fastforce
+
+lemma word_leq_minus_one_le:
+  fixes x :: "'a::len word"
+  shows "\<lbrakk>y \<noteq> 0; x \<le> y - 1 \<rbrakk> \<Longrightarrow> x < y"
+  using le_m1_iff_lt word_neq_0_conv by blast
+
+lemma word_count_from_top:
+  "n \<noteq> 0 \<Longrightarrow> {0 ..< n :: 'a :: len word} = {0 ..< n - 1} \<union> {n - 1}"
+  apply (rule set_eqI, rule iffI)
+   apply simp
+   apply (drule word_le_minus_one_leq)
+   apply (rule disjCI)
+   apply simp
+  apply simp
+  apply (erule word_leq_minus_one_le)
+  apply fastforce
+  done
+
+lemma word_minus_one_le_leq:
+  "\<lbrakk> x - 1 < y \<rbrakk> \<Longrightarrow> x \<le> (y :: 'a :: len word)"
+  apply (cases "x = 0")
+   apply simp
+  apply (simp add: word_less_nat_alt word_le_nat_alt)
+  apply (subst(asm) unat_minus_one)
+   apply (simp add: word_less_nat_alt)
+  apply (cases "unat x")
+   apply (simp add: unat_eq_zero)
+  apply arith
+  done
+
+lemma word_div_less:
+  "m < n \<Longrightarrow> m div n = 0" for m :: "'a :: len word"
+  by (simp add: unat_mono word_arith_nat_defs(6))
+
+lemma word_must_wrap:
+  "\<lbrakk> x \<le> n - 1; n \<le> x \<rbrakk> \<Longrightarrow> n = (0 :: 'a :: len word)"
+  using dual_order.trans sub_wrap word_less_1 by blast
+
+lemma range_subset_card:
+  "\<lbrakk> {a :: 'a :: len word .. b} \<subseteq> {c .. d}; b \<ge> a \<rbrakk> \<Longrightarrow> d \<ge> c \<and> d - c \<ge> b - a"
+  using word_sub_le word_sub_mono by fastforce
+
+lemma less_1_simp:
+  "n - 1 < m = (n \<le> (m :: 'a :: len word) \<and> n \<noteq> 0)"
+  by unat_arith
+
+lemma word_power_mod_div:
+  fixes x :: "'a::len word"
+  shows "\<lbrakk> n < LENGTH('a); m < LENGTH('a)\<rbrakk>
+  \<Longrightarrow> x mod 2 ^ n div 2 ^ m = x div 2 ^ m mod 2 ^ (n - m)"
+  apply (simp add: word_arith_nat_div unat_mod power_mod_div)
+  apply (subst unat_arith_simps(3))
+  apply (subst unat_mod)
+  apply (subst unat_of_nat)+
+  apply (simp add: mod_mod_power min.commute)
+  done
+
+lemma word_range_minus_1':
+  fixes a :: "'a :: len word"
+  shows "a \<noteq> 0 \<Longrightarrow> {a - 1<..b} = {a..b}"
+  by (simp add: greaterThanAtMost_def atLeastAtMost_def greaterThan_def atLeast_def less_1_simp)
+
+lemma word_range_minus_1:
+  fixes a :: "'a :: len word"
+  shows "b \<noteq> 0 \<Longrightarrow> {a..b - 1} = {a..<b}"
+  apply (simp add: atLeastLessThan_def atLeastAtMost_def atMost_def lessThan_def)
+  apply (rule arg_cong [where f = "\<lambda>x. {a..} \<inter> x"])
+  apply rule
+   apply clarsimp
+   apply (erule contrapos_pp)
+   apply (simp add: linorder_not_less linorder_not_le word_must_wrap)
+  apply (clarsimp)
+  apply (drule word_le_minus_one_leq)
+  apply (auto simp: word_less_sub_1)
+  done
+
+lemma ucast_nat_def:
+  "of_nat (unat x) = (ucast :: 'a :: len word \<Rightarrow> 'b :: len word) x"
+  by transfer simp
+
+lemma overflow_plus_one_self:
+  "(1 + p \<le> p) = (p = (-1 :: 'a :: len word))"
+  apply rule
+  apply (rule ccontr)
+   apply (drule plus_one_helper2)
+   apply (rule notI)
+   apply (drule arg_cong[where f="\<lambda>x. x - 1"])
+   apply simp
+   apply (simp add: field_simps)
+  apply simp
+  done
+
+lemma plus_1_less:
+  "(x + 1 \<le> (x :: 'a :: len word)) = (x = -1)"
+  apply (rule iffI)
+   apply (rule ccontr)
+   apply (cut_tac plus_one_helper2[where x=x, OF order_refl])
+    apply simp
+   apply clarsimp
+   apply (drule arg_cong[where f="\<lambda>x. x - 1"])
+   apply simp
+  apply simp
+  done
+
+lemma pos_mult_pos_ge:
+  "[|x > (0::int); n>=0 |] ==> n * x >= n*1"
+  apply (simp only: mult_left_mono)
+  done
+
+lemma word_plus_strict_mono_right:
+  fixes x :: "'a :: len word"
+  shows "\<lbrakk>y < z; x \<le> x + z\<rbrakk> \<Longrightarrow> x + y < x + z"
+  by unat_arith
+
+lemma word_div_mult:
+  "0 < c \<Longrightarrow> a < b * c \<Longrightarrow> a div c < b" for a b c :: "'a::len word"
+  by (rule classical)
+     (use div_to_mult_word_lt [of b a c] in
+      \<open>auto simp add: word_less_nat_alt word_le_nat_alt unat_div\<close>)
+
+lemma word_less_power_trans_ofnat:
+  "\<lbrakk>n < 2 ^ (m - k); k \<le> m; m < LENGTH('a)\<rbrakk>
+   \<Longrightarrow> of_nat n * 2 ^ k < (2::'a::len word) ^ m"
+  apply (subst mult.commute)
+  apply (rule word_less_power_trans)
+    apply (simp_all add: word_less_nat_alt less_le_trans take_bit_eq_mod)
+  done
+
+lemma word_1_le_power:
+  "n < LENGTH('a) \<Longrightarrow> (1 :: 'a :: len word) \<le> 2 ^ n"
+  by (rule inc_le[where i=0, simplified], erule iffD2[OF p2_gt_0])
+
+lemma unat_1_0:
+  "1 \<le> (x::'a::len word) = (0 < unat x)"
+  by (auto simp add: word_le_nat_alt)
+
+lemma x_less_2_0_1':
+  fixes x :: "'a::len word"
+  shows "\<lbrakk>LENGTH('a) \<noteq> 1; x < 2\<rbrakk> \<Longrightarrow> x = 0 \<or> x = 1"
+  apply (cases \<open>2 \<le> LENGTH('a)\<close>)
+  apply simp_all
+  apply transfer
+  apply auto
+  apply (metis add.commute add.right_neutral even_two_times_div_two mod_div_trivial mod_pos_pos_trivial mult.commute mult_zero_left not_less not_take_bit_negative odd_two_times_div_two_succ)
+  done
+
+lemmas word_add_le_iff2 = word_add_le_iff [folded no_olen_add_nat]
+
+lemma of_nat_power:
+  shows "\<lbrakk> p < 2 ^ x; x < len_of TYPE ('a) \<rbrakk> \<Longrightarrow> of_nat p < (2 :: 'a :: len word) ^ x"
+  apply (rule order_less_le_trans)
+   apply (rule of_nat_mono_maybe)
+    apply (erule power_strict_increasing)
+    apply simp
+   apply assumption
+  apply (simp add: word_unat_power del: of_nat_power)
+  done
+
+lemma of_nat_n_less_equal_power_2:
+  "n < LENGTH('a::len) \<Longrightarrow> ((of_nat n)::'a word) < 2 ^ n"
+  apply (induct n)
+   apply clarsimp
+  apply clarsimp
+  apply (metis of_nat_power n_less_equal_power_2 of_nat_Suc power_Suc)
+  done
+
+lemma eq_mask_less:
+  fixes w :: "'a::len word"
+  assumes eqm: "w = w AND mask n"
+  and      sz: "n < len_of TYPE ('a)"
+  shows "w < (2::'a word) ^ n"
+  by (subst eqm, rule and_mask_less' [OF sz])
+
+lemma of_nat_mono_maybe':
+  fixes Y :: "nat"
+  assumes xlt: "x < 2 ^ len_of TYPE ('a)"
+  assumes ylt: "y < 2 ^ len_of TYPE ('a)"
+  shows   "(y < x) = (of_nat y < (of_nat x :: 'a :: len word))"
+  apply (subst word_less_nat_alt)
+  apply (subst unat_of_nat)+
+  apply (subst mod_less)
+   apply (rule ylt)
+  apply (subst mod_less)
+   apply (rule xlt)
+  apply simp
+  done
+
+lemma of_nat_mono_maybe_le:
+  "\<lbrakk>x < 2 ^ LENGTH('a); y < 2 ^ LENGTH('a)\<rbrakk> \<Longrightarrow>
+  (y \<le> x) = ((of_nat y :: 'a :: len word) \<le> of_nat x)"
+  apply (clarsimp simp: le_less)
+  apply (rule disj_cong)
+   apply (rule of_nat_mono_maybe', assumption+)
+  apply auto
+  using of_nat_inj apply blast
+  done
+
+lemma mask_AND_NOT_mask:
+  "(w AND NOT (mask n)) AND mask n = 0"
+  for w :: \<open>'a::len word\<close>
+  by (rule bit_word_eqI) (simp add: bit_simps)
+
+lemma AND_NOT_mask_plus_AND_mask_eq:
+  "(w AND NOT (mask n)) + (w AND mask n) = w"
+  for w :: \<open>'a::len word\<close>
+  apply (subst disjunctive_add)
+  apply (auto simp add: bit_simps)
+  apply (rule bit_word_eqI)
+  apply (auto simp add: bit_simps)
+  done
+
+lemma mask_eqI:
+  fixes x :: "'a :: len word"
+  assumes m1: "x AND mask n = y AND mask n"
+  and     m2: "x AND NOT (mask n) = y AND NOT (mask n)"
+  shows "x = y"
+proof -
+  have *: \<open>x = x AND mask n OR x AND NOT (mask n)\<close> for x :: \<open>'a word\<close>
+    by (rule bit_word_eqI) (auto simp add: bit_simps)
+  from assms * [of x] * [of y] show ?thesis
+    by simp
+qed
+
+lemma neq_0_no_wrap:
+  fixes x :: "'a :: len word"
+  shows "\<lbrakk> x \<le> x + y; x \<noteq> 0 \<rbrakk> \<Longrightarrow> x + y \<noteq> 0"
+  by clarsimp
+
+lemma unatSuc2:
+  fixes n :: "'a :: len word"
+  shows "n + 1 \<noteq> 0 \<Longrightarrow> unat (n + 1) = Suc (unat n)"
+  by (simp add: add.commute unatSuc)
+
+lemma word_of_nat_le:
+  "n \<le> unat x \<Longrightarrow> of_nat n \<le> x"
+  apply (simp add: word_le_nat_alt unat_of_nat)
+  apply (erule order_trans[rotated])
+  apply (simp add: take_bit_eq_mod)
+  done
+
+lemma word_unat_less_le:
+  "a \<le> of_nat b \<Longrightarrow> unat a \<le> b"
+  by (metis eq_iff le_cases le_unat_uoi word_of_nat_le)
+
+lemma mask_Suc_0 : "mask (Suc 0) = (1 :: 'a::len word)"
+  by (simp add: mask_eq_decr_exp)
+
+lemma bool_mask':
+  fixes x :: "'a :: len word"
+  shows "2 < LENGTH('a) \<Longrightarrow> (0 < x AND 1) = (x AND 1 = 1)"
+  by (simp add: and_one_eq mod_2_eq_odd)
+
+lemma ucast_ucast_add:
+  fixes x :: "'a :: len word"
+  fixes y :: "'b :: len word"
+  shows
+  "LENGTH('b) \<ge> LENGTH('a) \<Longrightarrow>
+    ucast (ucast x + y) = x + ucast y"
+  apply transfer
+  apply simp
+  apply (subst (2) take_bit_add [symmetric])
+  apply (subst take_bit_add [symmetric])
+  apply simp
+  done
+
+lemma lt1_neq0:
+  fixes x :: "'a :: len word"
+  shows "(1 \<le> x) = (x \<noteq> 0)" by unat_arith
+
+lemma word_plus_one_nonzero:
+  fixes x :: "'a :: len word"
+  shows "\<lbrakk>x \<le> x + y; y \<noteq> 0\<rbrakk> \<Longrightarrow> x + 1 \<noteq> 0"
+  apply (subst lt1_neq0 [symmetric])
+  apply (subst olen_add_eqv [symmetric])
+  apply (erule word_random)
+  apply (simp add: lt1_neq0)
+  done
+
+lemma word_sub_plus_one_nonzero:
+  fixes n :: "'a :: len word"
+  shows "\<lbrakk>n' \<le> n; n' \<noteq> 0\<rbrakk> \<Longrightarrow> (n - n') + 1 \<noteq> 0"
+  apply (subst lt1_neq0 [symmetric])
+  apply (subst olen_add_eqv [symmetric])
+  apply (rule word_random [where x' = n'])
+   apply simp
+   apply (erule word_sub_le)
+  apply (simp add: lt1_neq0)
+  done
+
+lemma word_le_minus_mono_right:
+  fixes x :: "'a :: len word"
+  shows "\<lbrakk> z \<le> y; y \<le> x; z \<le> x \<rbrakk> \<Longrightarrow> x - y \<le> x - z"
+  apply (rule word_sub_mono)
+     apply simp
+    apply assumption
+   apply (erule word_sub_le)
+  apply (erule word_sub_le)
+  done
+
+lemma word_0_sle_from_less:
+  \<open>0 \<le>s x\<close> if \<open>x < 2 ^ (LENGTH('a) - 1)\<close> for x :: \<open>'a::len word\<close>
+  using that
+  apply transfer
+  apply (cases \<open>LENGTH('a)\<close>)
+   apply simp_all
+  apply (metis bit_take_bit_iff min_def nat_less_le not_less_eq take_bit_int_eq_self_iff take_bit_take_bit)
+  done
+
+lemma ucast_sub_ucast:
+  fixes x :: "'a::len word"
+  assumes "y \<le> x"
+  assumes T: "LENGTH('a) \<le> LENGTH('b)"
+  shows "ucast (x - y) = (ucast x - ucast y :: 'b::len word)"
+proof -
+  from T
+  have P: "unat x < 2 ^ LENGTH('b)" "unat y < 2 ^ LENGTH('b)"
+    by (fastforce intro!: less_le_trans[OF unat_lt2p])+
+  then show ?thesis
+    by (simp add: unat_arith_simps unat_ucast assms[simplified unat_arith_simps])
+qed
+
+lemma word_1_0:
+  "\<lbrakk>a + (1::('a::len) word) \<le> b; a < of_nat x\<rbrakk> \<Longrightarrow> a < b"
+  apply transfer
+  apply (subst (asm) take_bit_incr_eq)
+   apply (auto simp add: diff_less_eq)
+  using take_bit_int_less_exp le_less_trans by blast
+
+lemma unat_of_nat_less:"\<lbrakk> a < b; unat b = c \<rbrakk> \<Longrightarrow> a < of_nat c"
+  by fastforce
+
+lemma word_le_plus_1: "\<lbrakk> (y::('a::len) word) < y + n; a < n \<rbrakk> \<Longrightarrow> y + a \<le> y + a + 1"
+  by unat_arith
+
+lemma word_le_plus:"\<lbrakk>(a::('a::len) word) < a + b; c < b\<rbrakk> \<Longrightarrow> a \<le> a + c"
+  by (metis order_less_imp_le word_random)
+
+lemma sint_minus1 [simp]: "(sint x = -1) = (x = -1)"
+  apply (cases \<open>LENGTH('a)\<close>)
+   apply simp_all
+  apply transfer
+  apply (simp flip: signed_take_bit_eq_iff_take_bit_eq)
+  done
+
+lemma sint_0 [simp]: "(sint x = 0) = (x = 0)"
+  by (fact signed_eq_0_iff)
+
+(* It is not always that case that "sint 1 = 1", because of 1-bit word sizes.
+ * This lemma produces the different cases. *)
+lemma sint_1_cases:
+  P if \<open>\<lbrakk> len_of TYPE ('a::len) = 1; (a::'a word) = 0; sint a = 0 \<rbrakk> \<Longrightarrow> P\<close>
+     \<open>\<lbrakk> len_of TYPE ('a) = 1; a = 1; sint (1 :: 'a word) = -1 \<rbrakk> \<Longrightarrow> P\<close>
+     \<open>\<lbrakk> len_of TYPE ('a) > 1; sint (1 :: 'a word) = 1 \<rbrakk> \<Longrightarrow> P\<close>
+proof (cases \<open>LENGTH('a) = 1\<close>)
+  case True
+  then have \<open>a = 0 \<or> a = 1\<close>
+    by transfer auto
+  with True that show ?thesis
+    by auto
+next
+  case False
+  with that show ?thesis
+    by (simp add: less_le Suc_le_eq)
+qed
+
+lemma sint_int_min:
+  "sint (- (2 ^ (LENGTH('a) - Suc 0)) :: ('a::len) word) = - (2 ^ (LENGTH('a) - Suc 0))"
+  apply (cases \<open>LENGTH('a)\<close>)
+   apply simp_all
+  apply transfer
+  apply (simp add: signed_take_bit_int_eq_self)
+  done
+
+lemma sint_int_max_plus_1:
+  "sint (2 ^ (LENGTH('a) - Suc 0) :: ('a::len) word) = - (2 ^ (LENGTH('a) - Suc 0))"
+  apply (cases \<open>LENGTH('a)\<close>)
+   apply simp_all
+  apply (subst word_of_int_2p [symmetric])
+  apply (subst int_word_sint)
+  apply simp
+  done
+
+lemma uint_range':
+  \<open>0 \<le> uint x \<and> uint x < 2 ^ LENGTH('a)\<close>
+  for x :: \<open>'a::len word\<close>
+  by transfer simp
+
+lemma sint_of_int_eq:
+  "\<lbrakk> - (2 ^ (LENGTH('a) - 1)) \<le> x; x < 2 ^ (LENGTH('a) - 1) \<rbrakk> \<Longrightarrow> sint (of_int x :: ('a::len) word) = x"
+  by (simp add: signed_take_bit_int_eq_self)
+
+lemma of_int_sint:
+  "of_int (sint a) = a"
+  by simp
+
+lemma sint_ucast_eq_uint:
+    "\<lbrakk> \<not> is_down (ucast :: ('a::len word \<Rightarrow> 'b::len word)) \<rbrakk>
+            \<Longrightarrow> sint ((ucast :: ('a::len word \<Rightarrow> 'b::len word)) x) = uint x"
+  apply transfer
+  apply (simp add: signed_take_bit_take_bit)
+  done
+
+lemma word_less_nowrapI':
+  "(x :: 'a :: len word) \<le> z - k \<Longrightarrow> k \<le> z \<Longrightarrow> 0 < k \<Longrightarrow> x < x + k"
+  by uint_arith
+
+lemma mask_plus_1:
+  "mask n + 1 = (2 ^ n :: 'a::len word)"
+  by (clarsimp simp: mask_eq_decr_exp)
+
+lemma unat_inj: "inj unat"
+  by (metis eq_iff injI word_le_nat_alt)
+
+lemma unat_ucast_upcast:
+  "is_up (ucast :: 'b word \<Rightarrow> 'a word)
+      \<Longrightarrow> unat (ucast x :: ('a::len) word) = unat (x :: ('b::len) word)"
+  unfolding ucast_eq unat_eq_nat_uint
+  apply transfer
+  apply simp
+  done
+
+lemma ucast_mono:
+  "\<lbrakk> (x :: 'b :: len word) < y; y < 2 ^ LENGTH('a) \<rbrakk>
+   \<Longrightarrow> ucast x < ((ucast y) :: 'a :: len word)"
+  apply (simp only: flip: ucast_nat_def)
+  apply (rule of_nat_mono_maybe)
+  apply (rule unat_less_helper)
+  apply simp
+  apply (simp add: word_less_nat_alt)
+  done
+
+lemma ucast_mono_le:
+  "\<lbrakk>x \<le> y; y < 2 ^ LENGTH('b)\<rbrakk> \<Longrightarrow> (ucast (x :: 'a :: len word) :: 'b :: len word) \<le> ucast y"
+  apply (simp only: flip: ucast_nat_def)
+  apply (subst of_nat_mono_maybe_le[symmetric])
+    apply (rule unat_less_helper)
+    apply simp
+   apply (rule unat_less_helper)
+   apply (erule le_less_trans)
+  apply (simp_all add: word_le_nat_alt)
+  done
+
+lemma ucast_mono_le':
+  "\<lbrakk> unat y < 2 ^ LENGTH('b); LENGTH('b::len) < LENGTH('a::len); x \<le> y \<rbrakk>
+   \<Longrightarrow> ucast x \<le> (ucast y :: 'b word)" for x y :: \<open>'a::len word\<close>
+  by (auto simp: word_less_nat_alt intro: ucast_mono_le)
+
+lemma neg_mask_add_mask:
+  "((x:: 'a :: len word) AND NOT (mask n)) + (2 ^ n - 1) = x OR mask n"
+  unfolding mask_2pm1 [symmetric]
+  apply (subst word_plus_and_or_coroll; rule bit_word_eqI)
+   apply (auto simp add: bit_simps)
+  done
+
+lemma le_step_down_word:"\<lbrakk>(i::('a::len) word) \<le> n; i = n \<longrightarrow> P; i \<le> n - 1 \<longrightarrow> P\<rbrakk> \<Longrightarrow> P"
+  by unat_arith
+
+lemma le_step_down_word_2:
+  fixes x :: "'a::len word"
+  shows "\<lbrakk>x \<le>  y; x \<noteq> y\<rbrakk> \<Longrightarrow> x \<le> y - 1"
+  by (subst (asm) word_le_less_eq,
+      clarsimp,
+      simp add: word_le_minus_one_leq)
+
+lemma NOT_mask_AND_mask[simp]: "(w AND mask n) AND NOT (mask n) = 0"
+  by (clarsimp simp add: mask_eq_decr_exp Parity.bit_eq_iff bit_and_iff bit_not_iff bit_mask_iff)
+
+lemma and_and_not[simp]:"(a AND b) AND NOT b = 0"
+  for a b :: \<open>'a::len word\<close>
+  apply (subst word_bw_assocs(1))
+  apply clarsimp
+  done
+
+lemma ex_mask_1[simp]: "(\<exists>x. mask x = (1 :: 'a::len word))"
+  apply (rule_tac x=1 in exI)
+  apply (simp add:mask_eq_decr_exp)
+  done
+
+lemma not_switch:"NOT a = x \<Longrightarrow> a = NOT x"
+  by auto
+
+end
